coq-osiris/theories/proofmode/setup.v
@@ -39,7 +39,7 @@ Arguments extendfs δ !fps !fvs.
 Arguments eval η !e /.
 Arguments evals η !es /.
 Arguments evalfs η !fes /.
-Arguments eval_match deep η o !bs /.
+Arguments eval_match deep η !bs o /.
 Arguments eval_bindings η !bs /.
 Arguments eval_mexpr η !me /.
 Arguments eval_sitem ηδ !item /.
